src/M/Pluto/Language/Constant.lean
@@ -25,26 +25,27 @@ export ConstantT (I S T U B D)
 
 open ConstantT
 
-private def showWrapped (prefixTrue : String) (suffixTrue : String) (prefixFalse : String) (wrap : Bool) (x : String) : String :=
-  if wrap
-    then prefixTrue ++ x ++ suffixTrue
-    else prefixFalse ++ x
 
-private def mapWrapper'    := showWrapped "{"  "}" ","
-private def listWrapper'   := showWrapped "[" "]" ","
+mutual
 
-def showData (wrap : Bool): Data → String
-  | Data.Constr n []         => "sigma" ++ toString n ++ ".[]"
-  | Data.Constr n (f :: [])  => "sigma" ++ toString n ++ ".[" ++ showData true f ++ "]"
-  | Data.Constr n (f :: fs)  => "sigma" ++ toString n ++ ".[" ++ showData true f ++ showData false (Data.List fs) ++ "]"
-  | Data.Map  []             => "{}"
-  | Data.Map  ((p, q) :: []) => mapWrapper'  wrap $ showData true p ++ "=" ++ showData true q
-  | Data.Map  ((p, q) :: ps) => mapWrapper'  wrap $ showData true p ++ "=" ++ showData true q ++ showData false (Data.Map ps)
-  | Data.List []             => "[]"
-  | Data.List (x :: [])      => listWrapper' wrap $ showData true x
-  | Data.List (x :: xs)      => listWrapper' wrap $ showData true x ++ showData false (Data.List xs)
-  | Data.I    i              => toString i
-  | Data.B    b              => "0x" ++ toString b
+  def intercalateData : _root_.List Data → String
+    | []      => ""
+    | [x]     => showData x
+    | x :: xs => showData x ++ "," ++ intercalateData xs
+
+  def intercalateData' : _root_.List (Data × Data) → String
+    | []            => ""
+    | [(k, v)]      => showData k ++ "=" ++ showData v
+    | (k, v) :: kvs => showData k ++ "=" ++ showData v ++ "," ++ intercalateData' kvs
+
+  def showData : Data → String
+    | Data.Constr n fs => "sigma" ++ toString n ++ ".[" ++ intercalateData fs ++ "]"
+    | Data.Map  kvs    => "{" ++ intercalateData' kvs ++ "}"
+    | Data.List xs     => "[" ++ intercalateData xs ++ "]"
+    | Data.I    i      => toString i
+    | Data.B    b      => "0x" ++ toString b
+
+end
 
 instance : ToString (ConstantT ann) where
   toString : ConstantT ann → String
@@ -54,35 +55,7 @@ instance : ToString (ConstantT ann) where
     | U _       => "()"
     | B _ true  => "True"
     | B _ false => "False"
-    | D _ d     => "data " ++ showData true d
-
-example : toString (I () 3                                           ) = "3"        := rfl
-example : toString (S () $ ByteString.mk $ ByteArray.mk #[0xca, 0xfe]) = "0xcafe"   := rfl
-example : toString (T () "test"                                      ) = "\"test\"" := rfl
-example : toString (U ()                                             ) = "()"       := rfl
-example : toString (B () true                                        ) = "True"     := rfl
-example : toString (B () false                                       ) = "False"    := rfl
-
-private def testData :=
-  Data.List
-    [
-      Data.Map []
-    , Data.Map [
-        (Data.I 3, Data.List [])
-      ]
-    , Data.Map [
-        (Data.B $ ByteString.mk $ ByteArray.mk #[0xca, 0xfe], Data.List [Data.I 2])
-      ]
-    , Data.Map [
-        (Data.I 10, Data.I 20)
-      , (Data.I 30, Data.I 40)
-    ]
-    , Data.Constr 2 [Data.I 9, Data.I (-10)]
-    , Data.Constr 1 [Data.I (-11)]
-    , Data.Constr 0 []
-    ]
-
-#eval toString (D () testData) == "data [{},{3=[]},{0xcafe=[2]},{10=20,30=40},sigma2.[9,-10],sigma1.[-11],sigma0.[]]"
+    | D _ d     => "data " ++ showData d
 
 
 end Pluto.Language
