src/M/Pluto/Proof/AST.lean
@@ -7,10 +7,60 @@ open Pluto.Language
 open PlutusCore (ByteString Data)
 
 
+private def toString' (term : Term ann) : String :=
+  if hasSpace term
+    then "(" ++ toString term ++ ")"
+    else toString term
+
+
+attribute [local simp] toString toString' showTerm showTerm' showBinding showBindings showData intercalateData intercalateData'
+
+
+@[simp] theorem show_name : toString (Name.mk name) = name :=
+  by rfl
+
+
+@[simp] theorem show_ast_var : toString (Var ann name) = toString name :=
+  by simp
+
+
+@[simp] theorem show_ast_lambda : toString (Lambda ann names term) = "(\\" ++ intercalateName names ++ " -> " ++ toString term ++ ")" :=
+  by simp
+
+
+@[simp] theorem show_ast_apply : toString (Apply ann term term') = toString' term ++ " " ++ toString' term' :=
+  by simp
+
+
+@[simp] theorem show_ast_force : toString (Force ann term) = "! " ++ toString' term :=
+  by simp
+
+
+@[simp] theorem show_ast_delay : toString (Delay ann term) = "# " ++ toString' term :=
+  by simp
+
+
+@[simp] theorem show_ast_constant : toString (Constant ann cons) = toString cons :=
+  by simp
+
+
+@[simp] theorem show_ast_builtin : toString (Builtin ann builtin) = toString builtin :=
+  by simp
+  
+
+@[simp] theorem show_ast_let : toString (Let ann bindings term) = "let " ++ showBindings bindings ++ " in " ++ toString term :=
+  by simp
+
+
+@[simp] theorem show_ast_if : toString (IfThenElse ann term term' term'') = "if " ++ toString term ++ " then " ++ toString term' ++ " else " ++ toString term'' :=
+  by simp
+
+
 private def test01 : Term Unit :=
   Constant () $ I () 1
 
-example : toString test01 == "1" := rfl
+example : toString test01 = "1" :=
+  by rfl
 
 
 private def test02 : Term Unit :=
@@ -18,8 +68,8 @@ private def test02 : Term Unit :=
   Lambda () [x]
     $ Var () x
 
-theorem check02 : toString test02 == "(\\x -> x)" :=
-  by simp [toString, showTerm, test02]
+example : toString test02 = "(\\x -> x)" :=
+  by simp [test02]
 
 
 private def test03 : Term Unit :=
@@ -27,8 +77,8 @@ private def test03 : Term Unit :=
     [Binding () (Name.mk "x") $ Constant () $ I () 1]
     $ Constant () (I () 42)
 
-example : toString test03 == "let x = 1 in 42" :=
-  by simp [toString, showBinding, showBindings, showTerm, test03]
+example : toString test03 = "let x = 1 in 42" :=
+  by simp [test03]
 
 
 private def test04 : Term Unit :=
@@ -36,8 +86,8 @@ private def test04 : Term Unit :=
     [Binding () (Name.mk "id") test02]
     $ Constant () (I () 42)
 
-example : toString test04 == "let id = (\\x -> x) in 42" :=
-  by simp [toString, showTerm, test04, showBindings, showBinding, test02, check02]
+example : toString test04 = "let id = (\\x -> x) in 42" :=
+  by simp [test04, test02]
 
 
 private def test05 : Term Unit :=
@@ -48,8 +98,8 @@ private def test05 : Term Unit :=
       (Var () f)
       $ Constant () (I () 1)
 
-example : toString test05 == "let f = (\\x -> x) in f 1" :=
-  by simp [toString, showTerm, test05, showBindings, showBinding, test02, check02, intercalate', showTerm']
+example : toString test05 = "let f = (\\x -> x) in f 1" :=
+  by simp [test05, test02]
 
 
 private def test06 : Term Unit :=
@@ -67,8 +117,8 @@ private def test06 : Term Unit :=
     ]
     $ Var () res
 
-example : toString test06 == "let f = (\\x -> x); res = # (f 1) in res" :=
-  by simp [toString, showTerm, test06, showBindings, showBinding, test02, check02, intercalate', showTerm']
+example : toString test06 = "let f = (\\x -> x); res = # (f 1) in res" :=
+  by simp [test06, test02]
 
 
 private def test07 : Term Unit :=
@@ -87,8 +137,8 @@ private def test07 : Term Unit :=
     $ Force ()
     $ Var () res
 
-example : toString test07 == "let f = (\\x -> x); res = # (f 1) in ! res" :=
-  by simp [toString, showTerm, test07, showBindings, showBinding, test02, check02, intercalate', showTerm']
+example : toString test07 = "let f = (\\x -> x); res = # (f 1) in ! res" :=
+  by simp [test07, test02]
 
 
 private def test08 : Term Unit :=
@@ -116,52 +166,52 @@ private def test08 : Term Unit :=
       $ Delay ()
       $ Constant () (I () 7)
 
-example : toString test08 == "let iff = (\\cond x y -> if cond then x else y) in ! ((iff (# 42)) (# 7))" :=
-  by simp [toString, showTerm, test08, showBindings, showBinding, test02, check02, intercalate', showTerm']
+example : toString test08 = "let iff = (\\cond x y -> if cond then x else y) in ! ((iff (# 42)) (# 7))" :=
+  by simp [test08, test02]
 
 
-example : toString (Constant () $ B () true) == "True" := rfl
+example : toString (Constant () $ B () true) = "True" := rfl
 
 
-example : toString (Constant () $ B () false) == "False" := rfl
+example : toString (Constant () $ B () false) = "False" := rfl
 
 
-example : toString (Constant () $ I () 42) == "42" := rfl
+example : toString (Constant () $ I () 42) = "42" := rfl
 
 
-example : toString (Constant () $ I () (-2)) == "-2" := rfl
+example : toString (Constant () $ I () (-2)) = "-2" := rfl
 
 
-example : toString (Constant () $ S () $ ByteString.mk $ ByteArray.mk #[0x41]) == "0x41" := rfl
+example : toString (Constant () $ S () $ ByteString.mk $ ByteArray.mk #[0x41]) = "0x41" := rfl
 
 
-example : toString (Constant () $ T () "foobar") == "\"foobar\"" := rfl
+example : toString (Constant () $ T () "foobar") = "\"foobar\"" := rfl
 
 
-example : toString (Constant () $ U ()) == "()" := rfl
+example : toString (Constant () $ U ()) = "()" := rfl
 
 
-example : toString (Constant () $ D () $ Data.I 42) == "data 42" := rfl
+example : toString (Constant () $ D () $ Data.I 42) = "data 42" := rfl
 
 
-example : toString (Constant () $ D () $ Data.B $ ByteString.mk $ ByteArray.mk #[0x41]) == "data 0x41" := rfl
+example : toString (Constant () $ D () $ Data.B $ ByteString.mk $ ByteArray.mk #[0x41]) = "data 0x41" := rfl
 
 
-example : toString (Constant () $ D () $ Data.List [Data.I 1, Data.I 2, Data.I 3]) == "data [1,2,3]" :=
-  by simp [toString, showTerm, showData]
+example : toString (Constant () $ D () $ Data.List [Data.I 1, Data.I 2, Data.I 3]) = "data [1,2,3]" :=
+  by simp 
 
 
-example : toString (Constant () $ D () $ Data.List [Data.I 1, Data.B $ ByteString.mk $ ByteArray.mk #[0x41], Data.List [Data.I 42], Data.Map [(Data.B $ ByteString.mk $ ByteArray.mk #[0xfe], Data.I 7)]]) == "data [1,0x41,[42],{0xfe=7}]" :=
-  by simp [toString, showTerm, showData]
+example : toString (Constant () $ D () $ Data.List [Data.I 1, Data.B $ ByteString.mk $ ByteArray.mk #[0x41], Data.List [Data.I 42], Data.Map [(Data.B $ ByteString.mk $ ByteArray.mk #[0xfe], Data.I 7)]]) = "data [1,0x41,[42],{0xfe=7}]" :=
+  by simp
 
 
-example : toString (Constant () $ D () $ Data.Map [(Data.I 1, Data.B $ ByteString.mk $ ByteArray.mk #[0x42]), (Data.B $ ByteString.mk $ ByteArray.mk #[0xfe], Data.I 42),(Data.List [Data.I 1, Data.I 2], Data.List [Data.I 3, Data.I 4]),(Data.Map [(Data.I 1, Data.I 3)], Data.I 4)]) == "data {1=0x42,0xfe=42,[1,2]=[3,4],{1=3}=4}" :=
-  by simp [toString, showTerm, showData]
+example : toString (Constant () $ D () $ Data.Map [(Data.I 1, Data.B $ ByteString.mk $ ByteArray.mk #[0x42]), (Data.B $ ByteString.mk $ ByteArray.mk #[0xfe], Data.I 42),(Data.List [Data.I 1, Data.I 2], Data.List [Data.I 3, Data.I 4]),(Data.Map [(Data.I 1, Data.I 3)], Data.I 4)]) = "data {1=0x42,0xfe=42,[1,2]=[3,4],{1=3}=4}" :=
+  by simp
 
 
-example : toString (Constant () $ D () $ Data.Constr 0 [Data.I 1, Data.B $ ByteString.mk $ ByteArray.mk #[0x41]]) == "data sigma0.[1,0x41]" :=
-  by simp [toString, showTerm, showData]
+example : toString (Constant () $ D () $ Data.Constr 0 [Data.I 1, Data.B $ ByteString.mk $ ByteArray.mk #[0x41]]) = "data sigma0.[1,0x41]" :=
+  by simp
 
 
-example : toString (Program.mk $ Lambda () [Name.mk "x"] (Constant () $ I () 3)) == "(\\x -> 3)" :=
-  by simp [toString, showTerm]
+example : toString (Program.mk $ Lambda () [Name.mk "x"] (Constant () $ I () 3)) = "(\\x -> 3)" :=
+  by simp
