src/M/Pluto/Proof.lean
@@ -1,3 +1,4 @@
 
 
 import M.Pluto.Proof.AST
+import M.Pluto.Proof.Constant
